spi_model/SPI_schedulerScript.sml
@@ -7,10 +7,7 @@ val _ = new_theory "SPI_scheduler";
 (* X_ENABLE means X automaton is enabled for internal operation *)
 val INIT_ENABLE_def = Define `
 INIT_ENABLE (spi:spi_state) =
-((spi.init.state = init_reset) /\ 
-(spi.tx.state = tx_idle) /\
-(spi.rx.state = rx_idle) /\
-(spi.xfer.state = xfer_idle))`
+(spi.init.state = init_reset)`
 
 val TX_ENABLE_def = Define `
 TX_ENABLE (spi:spi_state) =
@@ -18,10 +15,7 @@ TX_ENABLE (spi:spi_state) =
 (spi.tx.state <> tx_conf_ready) /\ 
 (spi.tx.state <> tx_ready_for_trans) /\ 
 (spi.tx.state <> tx_trans_done) /\ 
-(spi.tx.state <> tx_channel_disabled) /\
-(spi.init.state = init_done) /\
-(spi.rx.state = rx_idle) /\
-(spi.xfer.state = xfer_idle))`
+(spi.tx.state <> tx_channel_disabled))`
 
 val RX_ENABLE_def = Define `
 RX_ENABLE (spi:spi_state) =
@@ -29,10 +23,7 @@ RX_ENABLE (spi:spi_state) =
 (spi.rx.state <> rx_conf_ready) /\ 
 (spi.rx.state <> rx_receive_data) /\
 (spi.rx.state <> rx_data_ready) /\ 
-(spi.rx.state <> rx_channel_disabled) /\
-(spi.init.state = init_done) /\
-(spi.tx.state = tx_idle) /\
-(spi.xfer.state = xfer_idle))`
+(spi.rx.state <> rx_channel_disabled))`
 
 val XFER_ENABLE_def = Define `
 XFER_ENABLE (spi:spi_state) =
@@ -41,10 +32,7 @@ XFER_ENABLE (spi:spi_state) =
 (spi.xfer.state <> xfer_ready_for_trans) /\
 (spi.xfer.state <> xfer_exchange_data) /\ 
 (spi.xfer.state <> xfer_data_ready) /\ 
-(spi.xfer.state <> xfer_channel_disabled) /\
-(spi.init.state = init_done) /\
-(spi.tx.state = tx_idle) /\
-(spi.rx.state = rx_idle))`
+(spi.xfer.state <> xfer_channel_disabled))`
 
 (* not used so far
 (* sheduler_cases: schedule -> spi_state -> spi_state *)
