driver_model/driver_callScript.sml
@@ -13,20 +13,24 @@ val call_tx_dr_def = Define `
 call_tx_dr (dr:driver_state) (buffer:word8 list) =
 dr with dr_tx := dr.dr_tx with
 <| state := dr_tx_idle;
-data_buf := buffer |>`
+data_buf := buffer;
+tx_left_length := LENGTH buffer |>`
 
 (* call_rx_dr: driver_state -> num -> driver_state *)
 val call_rx_dr_def = Define `
 call_rx_dr (dr:driver_state) (length: num) =
 dr with dr_rx := dr.dr_rx with
 <| state := dr_rx_idle;
-rx_left_length := length |>`
+rx_left_length := length;
+rx_data_buf := [] |>`
 
 (* call_xfer_dr: driver_state -> word8 list -> driver_state *)
 val call_xfer_dr_def = Define `
 call_xfer_dr (dr:driver_state) (buffer:word8 list) =
 dr with dr_xfer := dr.dr_xfer with
 <| state := dr_xfer_idle;
-xfer_dataOUT_buf := buffer |>`
+xfer_dataOUT_buf := buffer;
+xfer_dataIN_buf := [];
+xfer_left_length := LENGTH buffer|>`
 
 val _ = export_theory();
