thm/abs1_comb_hold_ref_relScript.sml
@@ -3,7 +3,7 @@ open SPI_stateTheory SPI_relationTheory;
 open driver_stateTheory driver_relationTheory;
 open ds_abs1_stateTheory;
 open ref_relTheory;
-open ds_abs1_relTheory SPI_txTheory ds_abs1_txTheory;
+open ds_abs1_relTheory;
 open abs1_comb_hold_ref_rel_call_lblTheory;
 open abs1_comb_hold_ref_rel_trans_lblTheory;
 
@@ -23,12 +23,43 @@ METIS_TAC [abs1_comb_hold_ref_rel_TX],
 METIS_TAC [abs1_comb_hold_ref_rel_RX],
 METIS_TAC [abs1_comb_hold_ref_rel_XFER]]);
 
+val abs1_comb_hold_ref_rel_driver_tr = store_thm("abs1_comb_hold_ref_rel_driver_tr",
+``!(spi:spi_state) (dr:driver_state) (ds_abs1:ds_abs1_state).
+(ref_rel ds_abs1 dr spi) /\ (driver_tr dr tau dr') ==>
+?ds_abs1'. (ds_abs1_tr ds_abs1 tau ds_abs1') /\ (ref_rel ds_abs1' dr' spi)``,
+cheat);
+
+val abs1_comb_hold_ref_rel_spi_tr = store_thm("abs1_comb_hold_ref_rel_spi_tr",
+``!(spi:spi_state) (dr:driver_state) (ds_abs1:ds_abs1_state).
+(ref_rel ds_abs1 dr spi) /\ (spi_tr spi tau spi') ==>
+?ds_abs1'. (ds_abs1_tr ds_abs1 tau ds_abs1') /\ (ref_rel ds_abs1' dr spi')``,
+cheat);
+
+val abs1_comb_hold_ref_rel_WR_UP = store_thm("abs1_comb_hold_ref_rel_WR_UP",
+``!(spi:spi_state) (dr:driver_state) (ds_abs1:ds_abs1_state).
+(ref_rel ds_abs1 dr spi) /\ (driver_tr dr (Write a v) dr') /\ 
+(spi_tr spi (Update a v) spi') ==>
+(ref_rel ds_abs1 dr' spi') \/
+(?ds_abs1'. (ds_abs1_tr ds_abs1 tau ds_abs1') /\ (ref_rel ds_abs1' dr' spi'))``,
+cheat);
+
+val abs1_comb_hold_ref_rel_RD_RE = store_thm("abs1_comb_hold_ref_rel_RD_RE",
+``!(spi:spi_state) (dr:driver_state) (ds_abs1:ds_abs1_state).
+(ref_rel ds_abs1 dr spi) /\ (driver_tr dr (Read a v) dr') /\ 
+(spi_tr spi (Return a v) spi') ==>
+(ref_rel ds_abs1 dr' spi')``,
+cheat);
+
 (* bi-simulation: ds_abs1 or ds_abs1' exists when lbl is tau *)
 val abs1_comb_hold_ref_rel_tau = store_thm("abs1_comb_hold_ref_rel_tau",
 ``!(spi:spi_state) (dr:driver_state) (ds_abs1:ds_abs1_state).
 (ref_rel ds_abs1 dr spi) /\ (local_tr (dr, spi) tau (dr', spi')) ==>
-(ref_rel ds_abs1 dr' spi') \/ (?ds_abs1'. (ds_abs1_tr ds_abs1 tau ds_abs1') \/ (ref_rel ds_abs1' dr' spi'))``,
-cheat);
+(ref_rel ds_abs1 dr' spi') \/ (?ds_abs1'. (ds_abs1_tr ds_abs1 tau ds_abs1') /\ (ref_rel ds_abs1' dr' spi'))``,
+rw [local_tr_cases] >|
+[METIS_TAC [abs1_comb_hold_ref_rel_driver_tr],
+METIS_TAC [abs1_comb_hold_ref_rel_spi_tr],
+METIS_TAC [abs1_comb_hold_ref_rel_WR_UP],
+METIS_TAC [abs1_comb_hold_ref_rel_RD_RE]]);
 
 (* bi-simulation ds_abs1 *)
 val abs1_comb_hold_ref_rel = store_thm("abs1_comb_hold_ref_rel",
@@ -52,37 +83,40 @@ rw [comb_abs1_hold_ref_rel_TX],
 rw [comb_abs1_hold_ref_rel_RX],
 rw [comb_abs1_hold_ref_rel_XFER]]);
 
+val comb_abs1_hold_ref_rel_tau_spi = store_thm("comb_abs1_hold_ref_rel_tau_spi",
+``!(spi:spi_state) (dr:driver_state) (ds_abs1:ds_abs1_state).
+(ref_rel ds_abs1 dr spi) /\ (ds_abs1_spi_tr ds_abs1 tau_spi ds_abs1') ==>
+?dr' spi'. (local_tr (dr, spi) tau (dr', spi')) /\ (ref_rel ds_abs1' dr' spi')``,
+cheat);
+
+val comb_abs1_hold_ref_rel_tau_dr = store_thm("comb_abs1_hold_ref_rel_tau_spi",
+``!(spi:spi_state) (dr:driver_state) (ds_abs1:ds_abs1_state).
+(ref_rel ds_abs1 dr spi) /\ (ds_abs1_dr_tr ds_abs1 tau_dr ds_abs1') ==>
+?dr' spi'. (local_tr (dr, spi) tau (dr', spi')) /\ (ref_rel ds_abs1' dr' spi')``,
+cheat);
+
+val comb_abs1_hold_ref_rel_tau_comb = store_thm("comb_abs1_hold_ref_rel_tau_comb",
+``!(spi:spi_state) (dr:driver_state) (ds_abs1:ds_abs1_state).
+(ref_rel ds_abs1 dr spi) /\ (ds_abs1_comb_tr ds_abs1 tau_comb ds_abs1') ==>
+?dr' spi'. (local_tr (dr, spi) tau (dr', spi')) /\ (ref_rel ds_abs1' dr' spi')``,
+cheat);
+
 (* bi-simulation (dr',spi') when lbl is tau *)
 val comb_abs1_hold_ref_rel_tau = store_thm("comb_abs1_hold_ref_rel_tau",
 ``!(spi:spi_state) (dr:driver_state) (ds_abs1:ds_abs1_state).
 (ref_rel ds_abs1 dr spi) /\ (ds_abs1_tr ds_abs1 tau ds_abs1') ==>
 ?dr' spi'. (local_tr (dr, spi) tau (dr', spi')) /\ (ref_rel ds_abs1' dr' spi')``,
-cheat);
+rw [ds_abs1_tr_cases] >|
+[METIS_TAC [comb_abs1_hold_ref_rel_tau_spi],
+METIS_TAC [comb_abs1_hold_ref_rel_tau_dr],
+METIS_TAC [comb_abs1_hold_ref_rel_tau_comb]]);
 
-<<<<<<< HEAD
-=======
-(* bi-simulation (dr',spi') when lbl is tau *)
-val comb_abs1_hold_ref_rel_tau = store_thm("comb_abs1_hold_ref_rel_tau",
-``!(spi:spi_state) (dr:driver_state) (ds_abs1:ds_abs1_state).
-(ref_rel ds_abs1 dr spi) /\ (ds_abs1_tr ds_abs1 tau ds_abs1') ==>
-?dr' spi'. (local_tr (dr, spi) tau (dr', spi')) /\ (ref_rel ds_abs1' dr' spi')``,
-cheat);
-
->>>>>>> 94c284a492b8db7f2ed64e29d103d306882860e9
 (* bi-simulation (dr, spi') *)
 val comb_abs1_hold_ref_rel = store_thm("comb_abs1_hold_ref_rel",
 ``!(spi:spi_state) (dr:driver_state) (ds_abs1:ds_abs1_state) (lbl:global_lbl_type).
 (ref_rel ds_abs1 dr spi) /\ (ds_abs1_tr ds_abs1 lbl ds_abs1') ==>
 (?dr' spi'. (local_tr (dr, spi) lbl (dr', spi')) /\ (ref_rel ds_abs1' dr' spi'))``,
 cheat);
-<<<<<<< HEAD
-=======
-
-
-
-
-
->>>>>>> 94c284a492b8db7f2ed64e29d103d306882860e9
 
 
 val _ = export_theory();
